src/lib/kernel/gemm/Kuiper.Kernel.GEMM.TensorCore2D.FadeUpdate.fsti
@@ -1,0 +1,46 @@
+module Kuiper.Kernel.GEMM.TensorCore2D.FadeUpdate
+
+#lang-pulse
+
+open Kuiper
+#set-options "--ifuel 1 --initial_fuel 0 --max_fuel 1"
+#set-options "--z3rlimit 120"
+
+open Kuiper.Array.Vectorized { has_vec_cpy, chunk }
+open Kuiper.EMatrix
+open Kuiper.Float16
+open Kuiper.Math { even, odd, even_2x, odd_2x1 }
+open Kuiper.Tensor
+open Kuiper.Array2.Strided
+open Kuiper.Tensor.Tiling
+open Kuiper.Tensor.Layout.Alg { l2_row_major as rm }
+open Kuiper.Kernel.GEMM.Copy.Vec2
+open Kuiper.Kernel.GEMM.Tiled.Common.Vec
+open Kuiper.Spec.GEMM
+open Kuiper.TensorCore
+open Pulse.Lib.Array
+open Pulse.Lib.Trade
+
+module Chest = Kuiper.Chest
+open Kuiper.Kernel.GEMM.TensorCore2D.FragmentAcc
+open Kuiper.Kernel.GEMM.TensorCore2D.Fade
+
+val lemma_update_tile_fade_comb_approximates
+  (#et : Type0) {| scalar et, real_like et|}
+  (ecomb : et -> et -> et)
+  (comb : real -> real -> real)
+  (tm tn wm wn : pos)
+  (idxI : natlt wm)
+  (idxJ : natlt wn)
+  (em : chest2 et (wm*tm) (wn*tn))
+  (etile : chest2 et tm tn)
+  (rm1 rm2 : chest2 real (wm*tm) (wn*tn))
+: Lemma
+  (requires
+    Kuiper.Approximates.approx2 ecomb comb /\
+    (em %~ (em_fade_comb_tiles comb tm tn wm wn idxI idxJ rm1 rm2)) /\
+    (etile %~ (ematrix_subtile rm2 tm tn idxI idxJ)))
+  (ensures
+    (update_tile em tm tn idxI idxJ
+      (Chest.chest_comb ecomb (ematrix_subtile em tm tn idxI idxJ) etile))
+    %~ (em_fade_comb_tiles comb tm tn wm wn idxI (idxJ + 1) rm1 rm2))
