src/lib/kernel/gemm/Kuiper.Kernel.GEMM.TensorCore2D.FragmentMMA.fst
@@ -1,0 +1,169 @@
+module Kuiper.Kernel.GEMM.TensorCore2D.FragmentMMA
+
+#lang-pulse
+
+open Kuiper
+#set-options "--ifuel 1 --initial_fuel 0 --max_fuel 1"
+#set-options "--z3rlimit 120"
+
+open Kuiper.Array.Vectorized { has_vec_cpy, chunk }
+open Kuiper.EMatrix
+open Kuiper.Float16
+open Kuiper.Math { even, odd, even_2x, odd_2x1 }
+open Kuiper.Tensor
+open Kuiper.Array2.Strided
+open Kuiper.Tensor.Tiling
+open Kuiper.Tensor.Layout.Alg { l2_row_major as rm }
+open Kuiper.Kernel.GEMM.Copy.Vec2
+open Kuiper.Kernel.GEMM.Tiled.Common.Vec
+open Kuiper.Spec.GEMM
+open Kuiper.TensorCore
+open Pulse.Lib.Array
+open Pulse.Lib.Trade
+
+open Kuiper.Kernel.GEMM.TensorCore2D.ProofSupport
+open Kuiper.Kernel.GEMM.TensorCore2D.FragmentAcc
+let arrayfragments_fade
+  (tm tn tk wm wn : szp)
+  (i : natlt wm)
+  (j : natlt wn)
+  (resIdxM : natle wm)
+  (resIdxN : natle wn)
+  (rA : chest2 real (wm*tm) tk)
+  (rB : chest2 real tk (wn*tn))
+  (rAcc : chest2 real (wm*tm) (wn*tn))
+: chest2 real tm tn
+=
+  if i < resIdxM || (i = resIdxM && j < resIdxN)
+  then ematrix_subtile rAcc tm tn i j `matplus`
+    (matmul (ematrix_subtile rA tm tk i 0) (ematrix_subtile rB tk tn 0 j))
+  else ematrix_subtile rAcc tm tn i j
+
+#push-options "--z3rlimit 80"
+inline_for_extraction noextract
+fn fragarray_mma
+  (#et_ab #et_acc : Type0)
+  {| scalar et_ab, scalar et_acc, real_like et_ab, real_like et_acc |}
+  (tm tn tk wm wn : szp)
+  (aFrags     : array (fragment et_ab FragA tm tn tk FragLRM))
+  (bFrags     : array (fragment et_ab FragB tm tn tk FragLRM))
+  (accumFrags : array (fragment et_acc FragAcc tm tn tk FragLAcc))
+  (rA : chest2 real (wm*tm) tk)
+  (rB : chest2 real tk (wn*tn))
+  (rAcc : chest2 real (wm*tm) (wn*tn))
+  (#_ : squash (Pulse.Lib.Array.length aFrags == wm))
+  (#_ : squash (Pulse.Lib.Array.length bFrags == wn))
+  (#_ : squash (Pulse.Lib.Array.length accumFrags == wm*wn))
+  preserves
+    fragarrayA_approximates wm aFrags rA **
+    fragarrayB_approximates wn bFrags rB
+  requires
+    pure (valid_frag_et_comb et_ab et_acc)
+  requires
+    fragarrayAcc_approximates wm wn accumFrags rAcc
+  ensures
+    fragarrayAcc_approximates wm wn accumFrags (rAcc `matplus` (matmul rA rB))
+{
+  unfold fragarrayA_approximates wm aFrags;
+  unfold fragarrayB_approximates wn bFrags;
+  unfold fragarrayAcc_approximates wm wn accumFrags;
+
+  with eAs. assert aFrags |-> eAs;
+  with eBs. assert bFrags |-> eBs;
+
+  let mut resIdxM = 0sz;
+  while (!resIdxM <^ wm)
+    invariant live resIdxM
+    invariant
+      exists* (eAcc : seq (chest2 et_acc tm tn)).
+        accumFrags |-> eAcc **
+        pure (
+          !resIdxM <= wm /\
+          (Seq.length eAcc == wm*wn) /\
+          forall (i : natlt wm) (j : natlt wn).
+            (Seq.index eAcc (i * wn + j)) %~
+              (arrayfragments_fade tm tn tk wm wn i j !resIdxM 0 rA rB rAcc))
+    decreases (wm - !resIdxM)
+  {
+    let mut resIdxN = 0sz;
+    while (!resIdxN <^ wn)
+      invariant live resIdxN
+      invariant
+        exists* (eAcc : seq (chest2 et_acc tm tn)).
+          accumFrags |-> eAcc **
+          pure (
+            !resIdxN <= wn /\
+            (Seq.length eAcc == wm*wn) /\
+            forall (i : natlt wm) (j : natlt wn).
+              (Seq.index eAcc (i * wn + j)) %~
+                (arrayfragments_fade tm tn tk wm wn i j !resIdxM !resIdxN rA rB rAcc))
+      decreases (wn - !resIdxN)
+    {
+      with eAccs. assert accumFrags |-> eAccs;
+
+      array_fragment_pts_to_ref aFrags;
+      array_fragment_pts_to_ref bFrags;
+      array_fragment_pts_to_ref accumFrags;
+
+      array_fragment_extract_ro aFrags !resIdxM;
+      array_fragment_extract_ro bFrags !resIdxN;
+      array_fragment_extract accumFrags (!resIdxM * wn + !resIdxN);
+
+      let a_frag = aFrags.(!resIdxM);
+      let b_frag = bFrags.(!resIdxN);
+      let acc_frag = accumFrags.(!resIdxM *^ wn +^ !resIdxN);
+
+      with eAt. assert a_frag |-> eAt;
+      with eBt. assert b_frag |-> eBt;
+      with eAcct. assert acc_frag |-> eAcct;
+      assert pure (eAt %~ (ematrix_subtile rA tm tk !resIdxM 0));
+      assert pure (eBt %~ (ematrix_subtile rB tk tn 0 !resIdxN));
+      assert pure (eAcct %~ (ematrix_subtile rAcc tm tn !resIdxM !resIdxN));
+
+      mma_sync' a_frag b_frag acc_frag;
+
+      Kuiper.TensorCore.Base.emma_approx_lemma eAcct eAt eBt
+        (ematrix_subtile rAcc tm tn !resIdxM !resIdxN)
+        (ematrix_subtile rA tm tk !resIdxM 0)
+        (ematrix_subtile rB tk tn 0 !resIdxN);
+
+      ambig_trade_elim ();
+      ambig_trade_elim ();
+
+      with v. assert acc_frag `fragment_pts_to` v;
+      Pulse.Lib.Forall.elim_forall v;
+
+      ambig_trade_elim ();
+
+      assert array_fragment_pts_to accumFrags (Seq.Base.upd eAccs
+            (!resIdxM * wn + !resIdxN)
+            (emma (Seq.index eAccs (!resIdxM * wn + !resIdxN))
+                (Seq.index eAs !resIdxM)
+                (Seq.index eBs !resIdxN)));
+
+      resIdxN := !resIdxN +^ 1sz;
+    };
+
+    resIdxM := !resIdxM +^ 1sz;
+  };
+
+  with eAcc. assert accumFrags |-> eAcc;
+  assert pure (
+    forall (i : natlt wm) (j : natlt wn).
+              (Seq.index eAcc (i * wn + j)) %~ (arrayfragments_fade tm tn tk wm wn i j wm 0 rA rB rAcc));
+  assert pure (
+    forall (i : natlt wm) (j : natlt wn).
+      (Seq.index eAcc (i * wn + j)) %~
+                ematrix_subtile rAcc tm tn i j `matplus`
+                  (matmul (ematrix_subtile rA tm tk i 0) (ematrix_subtile rB tk tn 0 j)));
+
+  assert pure (
+    forall (i : natlt wm) (j : natlt wn).
+              (Seq.index eAcc (i * wn + j)) %~ (ematrix_subtile (rAcc `matplus` (matmul rA rB)) tm tn i j));
+  assert pure (Seq.length eAcc == wm*wn);
+
+  fold fragarrayA_approximates wm aFrags rA;
+  fold fragarrayB_approximates wn bFrags rB;
+  fold fragarrayAcc_approximates wm wn accumFrags (rAcc `matplus` (matmul rA rB));
+}
+#pop-options
