src/lib/kernel/gemm/Kuiper.Kernel.GEMM.TensorCore2D.FragmentMMA.fsti
@@ -1,0 +1,51 @@
+module Kuiper.Kernel.GEMM.TensorCore2D.FragmentMMA
+
+#lang-pulse
+
+open Kuiper
+#set-options "--ifuel 1 --initial_fuel 0 --max_fuel 1"
+#set-options "--z3rlimit 120"
+
+open Kuiper.Array.Vectorized { has_vec_cpy, chunk }
+open Kuiper.EMatrix
+open Kuiper.Float16
+open Kuiper.Math { even, odd, even_2x, odd_2x1 }
+open Kuiper.Tensor
+open Kuiper.Array2.Strided
+open Kuiper.Tensor.Tiling
+open Kuiper.Tensor.Layout.Alg { l2_row_major as rm }
+open Kuiper.Kernel.GEMM.Copy.Vec2
+open Kuiper.Kernel.GEMM.Tiled.Common.Vec
+open Kuiper.Spec.GEMM
+open Kuiper.TensorCore
+open Pulse.Lib.Array
+open Pulse.Lib.Trade
+
+open Kuiper.Kernel.GEMM.TensorCore2D.ProofSupport
+open Kuiper.Kernel.GEMM.TensorCore2D.FragmentAcc
+
+#push-options "--z3rlimit 80"
+inline_for_extraction noextract
+fn fragarray_mma
+  (#et_ab #et_acc : Type0)
+  {| scalar et_ab, scalar et_acc, real_like et_ab, real_like et_acc |}
+  (tm tn tk wm wn : szp)
+  (aFrags     : array (fragment et_ab FragA tm tn tk FragLRM))
+  (bFrags     : array (fragment et_ab FragB tm tn tk FragLRM))
+  (accumFrags : array (fragment et_acc FragAcc tm tn tk FragLAcc))
+  (rA : chest2 real (wm*tm) tk)
+  (rB : chest2 real tk (wn*tn))
+  (rAcc : chest2 real (wm*tm) (wn*tn))
+  (#_ : squash (Pulse.Lib.Array.length aFrags == wm))
+  (#_ : squash (Pulse.Lib.Array.length bFrags == wn))
+  (#_ : squash (Pulse.Lib.Array.length accumFrags == wm*wn))
+  preserves
+    fragarrayA_approximates wm aFrags rA **
+    fragarrayB_approximates wn bFrags rB
+  requires
+    pure (valid_frag_et_comb et_ab et_acc)
+  requires
+    fragarrayAcc_approximates wm wn accumFrags rAcc
+  ensures
+    fragarrayAcc_approximates wm wn accumFrags (rAcc `matplus` (matmul rA rB))
+#pop-options
