src/lib/kernel/gemm/Kuiper.Kernel.GEMM.TensorCore2D.KernelLoop.fst
@@ -1,0 +1,336 @@
+module Kuiper.Kernel.GEMM.TensorCore2D.KernelLoop
+
+open Kuiper.Kernel.GEMM.TensorCore2D.KernelDesc { constraints }
+#lang-pulse
+
+open Kuiper
+#set-options "--ifuel 1 --initial_fuel 0 --max_fuel 1"
+#set-options "--z3rlimit 10"
+
+open Kuiper.Array.Vectorized { has_vec_cpy, chunk }
+open Kuiper.EMatrix
+open Kuiper.Math { even, odd, even_2x, odd_2x1 }
+open Kuiper.Tensor
+open Kuiper.Array2.Strided
+open Kuiper.Tensor.Tiling
+open Kuiper.Tensor.Layout.Alg { l2_row_major as rm }
+open Kuiper.Kernel.GEMM.Copy.Vec2
+open Kuiper.Kernel.GEMM.Tiled.Common.Vec
+open Kuiper.Spec.GEMM
+open Kuiper.TensorCore
+open Pulse.Lib.Array
+open Pulse.Lib.Trade
+
+module SZ = Kuiper.SizeT
+module B = Kuiper.Barrier
+module T = Kuiper.Tensor
+module FB = Kuiper.Kernel.GEMM.FlipFlopBarrier2
+module CV2 = Kuiper.Kernel.GEMM.Copy.Vec2
+module Chest = Kuiper.Chest
+module MU = Kuiper.Kernel.GEMM.Util
+
+open Kuiper.Kernel.GEMM.TensorCore2D.KernelDesc
+open Kuiper.Kernel.GEMM.TensorCore2D.FragmentAcc
+open Kuiper.Kernel.GEMM.TensorCore2D.Subproducts
+open Kuiper.Kernel.GEMM.TensorCore2D.KLoop
+
+let unfold_fb_contract () : FStar.Tactics.V2.Tac unit =
+  FStar.Tactics.V2.norm [delta_only [`%FB.contract]; iota; primops];
+  Pulse.Lib.Core.slprop_equiv_norm ()
+
+ghost
+fn bp_to_rin
+  (#etA #etB : Type0)
+  {| sized etA, has_vec_cpy etA, sized etB, has_vec_cpy etB |}
+  (#rows #shared #cols : pos)
+  (eA : chest2 etA rows shared)
+  (eB : chest2 etB shared cols)
+  (#bm : pos{bm /?+ rows}) (#bk : pos{bk /?+ shared}) (#bn : pos{bn /?+ cols})
+  (l1 : full_layout2 bm bk) (l2 : full_layout2 bk bn)
+  (sar1 : larray etA (bm * bk)) (sar2 : larray etB (bk * bn))
+  (sa1 : array2 etA l1) (sa2 : array2 etB l2)
+  (nthr : pos) (bid : natlt (rows/bm * (cols/bn)))
+  (it : nat) (tid : natlt nthr)
+  requires
+    FB.barrier_p eA eB sa1 sa2 nthr bid it tid **
+    pure (sa1 == from_array l1 sar1 /\ sa2 == from_array l2 sar2)
+  ensures
+    (FB.contract eA eB l1 l2 sar1 sar2 nthr bid).rin it tid
+{
+  rewrite each sa1 as (from_array l1 sar1);
+  rewrite each sa2 as (from_array l2 sar2);
+  rewrite FB.barrier_p eA eB (from_array l1 sar1) (from_array l2 sar2) nthr bid it tid
+       as (FB.contract eA eB l1 l2 sar1 sar2 nthr bid).rin it tid
+       by unfold_fb_contract ();
+}
+
+ghost
+fn rout_to_bq
+  (#etA #etB : Type0)
+  {| sized etA, has_vec_cpy etA, sized etB, has_vec_cpy etB |}
+  (#rows #shared #cols : pos)
+  (eA : chest2 etA rows shared)
+  (eB : chest2 etB shared cols)
+  (#bm : pos{bm /?+ rows}) (#bk : pos{bk /?+ shared}) (#bn : pos{bn /?+ cols})
+  (l1 : full_layout2 bm bk) (l2 : full_layout2 bk bn)
+  (sar1 : larray etA (bm * bk)) (sar2 : larray etB (bk * bn))
+  (sa1 : array2 etA l1) (sa2 : array2 etB l2)
+  (nthr : pos) (bid : natlt (rows/bm * (cols/bn)))
+  (it : nat) (tid : natlt nthr)
+  requires
+    (FB.contract eA eB l1 l2 sar1 sar2 nthr bid).rout it tid **
+    pure (sa1 == from_array l1 sar1 /\ sa2 == from_array l2 sar2)
+  ensures
+    FB.barrier_q eA eB sa1 sa2 nthr bid it tid
+{
+  rewrite (FB.contract eA eB l1 l2 sar1 sar2 nthr bid).rout it tid
+       as FB.barrier_q eA eB (from_array l1 sar1) (from_array l2 sar2) nthr bid it tid
+       by unfold_fb_contract ();
+  rewrite each (from_array l1 sar1) as sa1;
+  rewrite each (from_array l2 sar2) as sa2;
+}
+
+#push-options "--fuel 0 --ifuel 0 --z3rlimit 20"
+let lemma_double_div (k bk : pos)
+  : Lemma (requires bk /?+ k)
+          (ensures 2 * k / bk == 2 * (k / bk))
+  = Kuiper.Divides.lemma_nat_divides_pos_divides bk k;
+    assert (bk * (k / bk) == k);
+    FStar.Math.Lemmas.cancel_mul_div (2 * (k / bk)) bk
+
+let double_succ (x : nat) : Lemma (2 * (x + 1) == 2 * x + 2) = ()
+
+let le_not_lt_eq (x y : nat)
+  : Lemma (requires x <= y /\ ~(x < y)) (ensures x == y)
+  = ()
+#pop-options
+
+ghost
+fn advance_barrier_state
+  (x : nat)
+  (next : nat { next == x + 1 })
+  requires B.barrier_state (2 * x + 1 + 1)
+  ensures B.barrier_state (2 * next)
+{
+  rewrite B.barrier_state (2 * x + 1 + 1)
+       as B.barrier_state (2 * next);
+}
+
+#push-options "--fuel 1 --ifuel 1 --z3rlimit 10"
+inline_for_extraction noextract
+fn run_loop
+  (#et_ab #et_c : Type0)
+  {| scalar et_ab, has_vec_cpy et_ab, scalar et_c |}
+  {| real_like et_ab, real_like et_c |}
+  (#m #n #k : szp)
+  (#lA : layout2 m k) {| T.ctlayout lA |}
+  (gA : array2 et_ab lA)
+  (#eA : chest2 et_ab m k)
+  (#lB : layout2 k n) {| T.ctlayout lB |}
+  {| str_A : strided_row_major lA,
+     str_B : strided_row_major lB |}
+  (#_ : squash (aligned_strided_row_major (chunk et_ab) str_A))
+  (#_ : squash (aligned_strided_row_major (chunk et_ab) str_B))
+  (gB : array2 et_ab lB)
+  (#eB : chest2 et_ab k n)
+  (bm bn bk tm tn tk wm wn : szp {
+    constraints bm bn bk tm tn tk wm wn })
+  (#_ : squash (bm /?+ m))
+  (#_ : squash (bn /?+ n))
+  (#_ : squash (bk /?+ k))
+  (#_ : squash (SZ.fits (bm * bk) /\ SZ.fits (bk * bn)))
+  (#_ : squash (chunk et_ab /?+ bn))
+  (#_ : squash (chunk et_ab /?+ bk))
+  (#_ : squash (SZ.fits (m * k)))
+  (#_ : squash (SZ.fits (k * n)))
+  (#_ : squash (SZ.fits (wm * tm)))
+  (#_ : squash (SZ.fits (wn * tn)))
+  (#_ : squash (valid_frag_et_dims et_ab FragA tm tn tk))
+  (#_ : squash (valid_frag_et_dims et_ab FragB tm tn tk))
+  (#_ : squash (valid_frag_et_dims et_c FragAcc tm tn tk))
+  (#_ : squash (valid_frag_et_comb et_ab et_c))
+  (#_ : squash (wm * tm /?+ m))
+  (#_ : squash (wn * tn /?+ n))
+  (#fA #fB : perm)
+  (rA : chest2 real m k)
+  (rB : chest2 real k n)
+  (mapA mapB : real -> real)
+  (emA emB : et_ab -> et_ab)
+  (#_ : squash (MU.approx1 emA mapA))
+  (#_ : squash (MU.approx1 emB mapB))
+  (nthr : erased nat {
+    nthr == bm/(wm*tm) * (bn/(wn*tn)) * warp_size })
+  (#_ : squash (chunk et_ab * nthr /?+ (bm * bk)))
+  (#_ : squash (chunk et_ab * nthr /?+ (bk * bn)))
+  (#_ : squash (SZ.fits (bm * bk + nthr - 1)))
+  (#_ : squash (SZ.fits (bk * bn + nthr - 1)))
+  (sarA : larray et_ab (bm * bk))
+  (sarB : larray et_ab (bk * bn))
+  (sA : array2 et_ab (rm bm bk))
+  (sB : array2 et_ab (rm bk bn))
+  (#_ : squash (
+    sA == from_array (rm bm bk) sarA /\
+    sB == from_array (rm bk bn) sarB))
+  (bid : szlt (m/bm * (n/bn)))
+  (tid : szlt nthr)
+  (mrow : szlt (m/bm) {
+    SZ.v mrow == SZ.v bid / (SZ.v n / SZ.v bn) })
+  (mcol : szlt (n/bn) {
+    SZ.v mcol == SZ.v bid % (SZ.v n / SZ.v bn) })
+  (warpRow : szlt (bm/(wm*tm)))
+  (warpCol : szlt (bn/(wn*tn)))
+  (gwRow : enatlt (m/(wm*tm)) {
+    gwRow == mrow * (bm/(wm*tm)) + warpRow })
+  (gwCol : enatlt (n/(wn*tn)) {
+    gwCol == mcol * (bn/(wn*tn)) + warpCol })
+  (rAcc0 : chest2 real (wm*tm) (wn*tn) {
+    rAcc0 == const _ 0.0R })
+  (aFrags : array (fragment et_ab FragA tm tn tk FragLRM))
+  (bFrags : array (fragment et_ab FragB tm tn tk FragLRM))
+  (accFrags : array (fragment et_c FragAcc tm tn tk FragLAcc))
+  (#_ : squash (Pulse.Lib.Array.length aFrags == wm))
+  (#_ : squash (Pulse.Lib.Array.length bFrags == wn))
+  (#_ : squash (Pulse.Lib.Array.length accFrags == wm * wn))
+  ()
+  preserves
+    gpu **
+    gA |-> Frac (fA /. (m/bm * (n/bn) * nthr)) eA **
+    gB |-> Frac (fB /. (m/bm * (n/bn) * nthr)) eB **
+    thread_id nthr tid **
+    block_id (m/bm * (n/bn)) bid **
+    B.barrier_tok
+      (FB.contract eA eB (rm bm bk) (rm bk bn) sarA sarB nthr bid) **
+    live aFrags **
+    live bFrags
+  requires
+    pure (aligned 16 (core gA)) **
+    pure (aligned 16 (core gB)) **
+    pure (eA %~ rA /\ eB %~ rB) **
+    fragarrayAcc_approximates wm wn accFrags
+      (kacc_inv m n k bm bn bk tm tn tk wm wn
+        (Chest.chest_map mapA rA) (Chest.chest_map mapB rB)
+        rAcc0 gwRow gwCol 0) **
+    (exists* em1. FB.bp_sharing sA em1 nthr) **
+    (exists* em2. FB.bp_sharing sB em2 nthr) **
+    B.barrier_state 0
+  ensures
+    fragarrayAcc_approximates wm wn accFrags
+      (kacc_inv m n k bm bn bk tm tn tk wm wn
+        (Chest.chest_map mapA rA) (Chest.chest_map mapB rB)
+        rAcc0 gwRow gwCol (k / bk)) **
+    (exists* em1. FB.bp_sharing sA em1 nthr) **
+    (exists* em2. FB.bp_sharing sB em2 nthr) **
+    B.barrier_state (2 * (k / bk))
+{
+  let num_k_tiles = k /^ bk;
+  let mut bkIdx : sz = 0sz;
+  while (!bkIdx <^ num_k_tiles)
+    invariant
+      exists* (vbkIdx : sz { vbkIdx <= num_k_tiles }).
+        bkIdx |-> vbkIdx **
+        fragarrayAcc_approximates wm wn accFrags
+          (kacc_inv m n k bm bn bk tm tn tk wm wn
+            (Chest.chest_map mapA rA) (Chest.chest_map mapB rB)
+            rAcc0 gwRow gwCol !bkIdx)
+    invariant live aFrags ** live bFrags
+    invariant
+      (exists* em1. FB.bp_sharing sA em1 nthr) **
+      (exists* em2. FB.bp_sharing sB em2 nthr) **
+      B.barrier_state (2 * !bkIdx)
+    decreases (num_k_tiles - !bkIdx)
+  {
+    even_2x !bkIdx;
+    assert pure ((2 * !bkIdx % 2 = 0) == true);
+    assert pure (even (2 * !bkIdx));
+
+    FB.fold_barrier_p_even eA eB sA sB nthr bid !bkIdx tid;
+    bp_to_rin eA eB (rm bm bk) (rm bk bn)
+      sarA sarB sA sB nthr bid (2 * !bkIdx) tid;
+    B.barrier_wait ();
+    rout_to_bq eA eB (rm bm bk) (rm bk bn)
+      sarA sarB sA sB nthr bid (2 * !bkIdx) tid;
+    FB.unfold_barrier_q_even eA eB sA sB nthr bid !bkIdx tid;
+
+    unfold FB.live_strided_chunks sA nthr tid;
+    with eA0. assert (FB.own_strided_chunks sA eA0 nthr tid);
+    rewrite FB.own_strided_chunks sA eA0 nthr tid
+      as CV2.own_strided_chunks sA eA0 nthr tid;
+    fold CV2.live_strided_chunks sA nthr tid;
+    unfold FB.live_strided_chunks sB nthr tid;
+    with eB0. assert (FB.own_strided_chunks sB eB0 nthr tid);
+    rewrite FB.own_strided_chunks sB eB0 nthr tid
+      as CV2.own_strided_chunks sB eB0 nthr tid;
+    fold CV2.live_strided_chunks sB nthr tid;
+
+    copy_tiles_out_of_matrices_vec bm bn bk sA sB gA gB
+      mrow !bkIdx mcol
+      (bm/^(wm*^tm)*^(bn/^(wn*^tn))*^warp_size) tid;
+
+    rewrite CV2.own_strided_chunks sA
+      (ematrix_subtile eA bm bk mrow !bkIdx) nthr tid
+      as FB.own_strided_chunks sA
+        (ematrix_subtile eA bm bk mrow !bkIdx) nthr tid;
+    rewrite CV2.own_strided_chunks sB
+      (ematrix_subtile eB bk bn !bkIdx mcol) nthr tid
+      as FB.own_strided_chunks sB
+        (ematrix_subtile eB bk bn !bkIdx mcol) nthr tid;
+
+    odd_2x1 !bkIdx;
+    assert pure (odd (2 * !bkIdx + 1));
+    FB.fold_barrier_p_odd eA eB sA sB nthr bid mrow mcol !bkIdx tid;
+    bp_to_rin eA eB (rm bm bk) (rm bk bn)
+      sarA sarB sA sB nthr bid (2 * !bkIdx + 1) tid;
+    B.barrier_wait ();
+
+    even_2x (!bkIdx + 1);
+    lemma_double_div (SZ.v k) (SZ.v bk);
+    double_succ !bkIdx;
+    assert pure (odd (2 * !bkIdx + 1));
+    assert pure ((2 * !bkIdx + 1) < 2 * k / bk);
+    assert pure (even (2 * !bkIdx + 2));
+    rout_to_bq eA eB (rm bm bk) (rm bk bn)
+      sarA sarB sA sB nthr bid (2 * !bkIdx + 1) tid;
+    FB.unfold_barrier_q_odd eA eB sA sB nthr bid mrow mcol !bkIdx tid;
+
+    unfold FB.bp_sharing sA
+      (ematrix_subtile eA bm bk mrow !bkIdx) nthr;
+    unfold FB.bp_sharing sB
+      (ematrix_subtile eB bk bn !bkIdx mcol) nthr;
+
+    let rA_sub = ematrix_subtile rA bm bk mrow !bkIdx;
+    let rB_sub = ematrix_subtile rB bk bn !bkIdx mcol;
+    let vbk = !bkIdx;
+    subtile_approx eA rA bm bk mrow vbk;
+    subtile_approx eB rB bk bn vbk mcol;
+
+    ktile_advance
+      m n k bm bn bk tm tn tk wm wn
+      aFrags bFrags accFrags sA sB rA rB
+      mrow mcol vbk rA_sub rB_sub
+      emA emB mapA mapB rAcc0
+      warpRow warpCol gwRow gwCol ();
+
+    fold FB.bp_sharing sA
+      (ematrix_subtile eA bm bk mrow !bkIdx) nthr;
+    fold FB.bp_sharing sB
+      (ematrix_subtile eB bk bn !bkIdx mcol) nthr;
+
+    let next_bkIdx = !bkIdx +^ 1sz;
+    advance_barrier_state (SZ.v !bkIdx) (SZ.v next_bkIdx);
+    bkIdx := next_bkIdx;
+  };
+
+  assert pure (SZ.v num_k_tiles == k / bk);
+  le_not_lt_eq (SZ.v !bkIdx) (SZ.v num_k_tiles);
+  rewrite fragarrayAcc_approximates wm wn accFrags
+      (kacc_inv m n k bm bn bk tm tn tk wm wn
+        (Chest.chest_map mapA rA) (Chest.chest_map mapB rB)
+        rAcc0 gwRow gwCol !bkIdx)
+    as fragarrayAcc_approximates wm wn accFrags
+      (kacc_inv m n k bm bn bk tm tn tk wm wn
+        (Chest.chest_map mapA rA) (Chest.chest_map mapB rB)
+        rAcc0 gwRow gwCol (k / bk));
+  rewrite B.barrier_state (2 * !bkIdx)
+       as B.barrier_state (2 * (k / bk));
+}
+#pop-options
