src/lib/kernel/gemm/Kuiper.Kernel.GEMM.TensorCore2D.KernelLoop.fsti
@@ -1,0 +1,141 @@
+module Kuiper.Kernel.GEMM.TensorCore2D.KernelLoop
+
+open Kuiper.Kernel.GEMM.TensorCore2D.KernelDesc { constraints }
+#lang-pulse
+
+open Kuiper
+#set-options "--ifuel 1 --initial_fuel 0 --max_fuel 1"
+#set-options "--z3rlimit 10"
+
+open Kuiper.Array.Vectorized { has_vec_cpy, chunk }
+open Kuiper.EMatrix
+open Kuiper.Math { even, odd, even_2x, odd_2x1 }
+open Kuiper.Tensor
+open Kuiper.Array2.Strided
+open Kuiper.Tensor.Tiling
+open Kuiper.Tensor.Layout.Alg { l2_row_major as rm }
+open Kuiper.Kernel.GEMM.Copy.Vec2
+open Kuiper.Kernel.GEMM.Tiled.Common.Vec
+open Kuiper.Spec.GEMM
+open Kuiper.TensorCore
+open Pulse.Lib.Array
+open Pulse.Lib.Trade
+
+module SZ = Kuiper.SizeT
+module B = Kuiper.Barrier
+module T = Kuiper.Tensor
+module FB = Kuiper.Kernel.GEMM.FlipFlopBarrier2
+module Chest = Kuiper.Chest
+module MU = Kuiper.Kernel.GEMM.Util
+
+open Kuiper.Kernel.GEMM.TensorCore2D.KernelDesc
+open Kuiper.Kernel.GEMM.TensorCore2D.FragmentAcc
+open Kuiper.Kernel.GEMM.TensorCore2D.Subproducts
+open Kuiper.Kernel.GEMM.TensorCore2D.KLoop
+
+#push-options "--fuel 1 --ifuel 1 --z3rlimit 10"
+inline_for_extraction noextract
+fn run_loop
+  (#et_ab #et_c : Type0)
+  {| scalar et_ab, has_vec_cpy et_ab, scalar et_c |}
+  {| real_like et_ab, real_like et_c |}
+  (#m #n #k : szp)
+  (#lA : layout2 m k) {| T.ctlayout lA |}
+  (gA : array2 et_ab lA)
+  (#eA : chest2 et_ab m k)
+  (#lB : layout2 k n) {| T.ctlayout lB |}
+  {| str_A : strided_row_major lA,
+     str_B : strided_row_major lB |}
+  (#_ : squash (aligned_strided_row_major (chunk et_ab) str_A))
+  (#_ : squash (aligned_strided_row_major (chunk et_ab) str_B))
+  (gB : array2 et_ab lB)
+  (#eB : chest2 et_ab k n)
+  (bm bn bk tm tn tk wm wn : szp {
+    constraints bm bn bk tm tn tk wm wn })
+  (#_ : squash (bm /?+ m))
+  (#_ : squash (bn /?+ n))
+  (#_ : squash (bk /?+ k))
+  (#_ : squash (SZ.fits (bm * bk) /\ SZ.fits (bk * bn)))
+  (#_ : squash (chunk et_ab /?+ bn))
+  (#_ : squash (chunk et_ab /?+ bk))
+  (#_ : squash (SZ.fits (m * k)))
+  (#_ : squash (SZ.fits (k * n)))
+  (#_ : squash (SZ.fits (wm * tm)))
+  (#_ : squash (SZ.fits (wn * tn)))
+  (#_ : squash (valid_frag_et_dims et_ab FragA tm tn tk))
+  (#_ : squash (valid_frag_et_dims et_ab FragB tm tn tk))
+  (#_ : squash (valid_frag_et_dims et_c FragAcc tm tn tk))
+  (#_ : squash (valid_frag_et_comb et_ab et_c))
+  (#_ : squash (wm * tm /?+ m))
+  (#_ : squash (wn * tn /?+ n))
+  (#fA #fB : perm)
+  (rA : chest2 real m k)
+  (rB : chest2 real k n)
+  (mapA mapB : real -> real)
+  (emA emB : et_ab -> et_ab)
+  (#_ : squash (MU.approx1 emA mapA))
+  (#_ : squash (MU.approx1 emB mapB))
+  (nthr : erased nat {
+    nthr == bm/(wm*tm) * (bn/(wn*tn)) * warp_size })
+  (#_ : squash (chunk et_ab * nthr /?+ (bm * bk)))
+  (#_ : squash (chunk et_ab * nthr /?+ (bk * bn)))
+  (#_ : squash (SZ.fits (bm * bk + nthr - 1)))
+  (#_ : squash (SZ.fits (bk * bn + nthr - 1)))
+  (sarA : larray et_ab (bm * bk))
+  (sarB : larray et_ab (bk * bn))
+  (sA : array2 et_ab (rm bm bk))
+  (sB : array2 et_ab (rm bk bn))
+  (#_ : squash (
+    sA == from_array (rm bm bk) sarA /\
+    sB == from_array (rm bk bn) sarB))
+  (bid : szlt (m/bm * (n/bn)))
+  (tid : szlt nthr)
+  (mrow : szlt (m/bm) {
+    SZ.v mrow == SZ.v bid / (SZ.v n / SZ.v bn) })
+  (mcol : szlt (n/bn) {
+    SZ.v mcol == SZ.v bid % (SZ.v n / SZ.v bn) })
+  (warpRow : szlt (bm/(wm*tm)))
+  (warpCol : szlt (bn/(wn*tn)))
+  (gwRow : enatlt (m/(wm*tm)) {
+    gwRow == mrow * (bm/(wm*tm)) + warpRow })
+  (gwCol : enatlt (n/(wn*tn)) {
+    gwCol == mcol * (bn/(wn*tn)) + warpCol })
+  (rAcc0 : chest2 real (wm*tm) (wn*tn) {
+    rAcc0 == const _ 0.0R })
+  (aFrags : array (fragment et_ab FragA tm tn tk FragLRM))
+  (bFrags : array (fragment et_ab FragB tm tn tk FragLRM))
+  (accFrags : array (fragment et_c FragAcc tm tn tk FragLAcc))
+  (#_ : squash (Pulse.Lib.Array.length aFrags == wm))
+  (#_ : squash (Pulse.Lib.Array.length bFrags == wn))
+  (#_ : squash (Pulse.Lib.Array.length accFrags == wm * wn))
+  ()
+  preserves
+    gpu **
+    gA |-> Frac (fA /. (m/bm * (n/bn) * nthr)) eA **
+    gB |-> Frac (fB /. (m/bm * (n/bn) * nthr)) eB **
+    thread_id nthr tid **
+    block_id (m/bm * (n/bn)) bid **
+    B.barrier_tok
+      (FB.contract eA eB (rm bm bk) (rm bk bn) sarA sarB nthr bid) **
+    live aFrags **
+    live bFrags
+  requires
+    pure (aligned 16 (core gA)) **
+    pure (aligned 16 (core gB)) **
+    pure (eA %~ rA /\ eB %~ rB) **
+    fragarrayAcc_approximates wm wn accFrags
+      (kacc_inv m n k bm bn bk tm tn tk wm wn
+        (Chest.chest_map mapA rA) (Chest.chest_map mapB rB)
+        rAcc0 gwRow gwCol 0) **
+    (exists* em1. FB.bp_sharing sA em1 nthr) **
+    (exists* em2. FB.bp_sharing sB em2 nthr) **
+    B.barrier_state 0
+  ensures
+    fragarrayAcc_approximates wm wn accFrags
+      (kacc_inv m n k bm bn bk tm tn tk wm wn
+        (Chest.chest_map mapA rA) (Chest.chest_map mapB rB)
+        rAcc0 gwRow gwCol (k / bk)) **
+    (exists* em1. FB.bp_sharing sA em1 nthr) **
+    (exists* em2. FB.bp_sharing sB em2 nthr) **
+    B.barrier_state (2 * (k / bk))
+#pop-options
