src/lib/kernel/gemm/Kuiper.Kernel.GEMM.TensorCore2D.ProofSupport.fsti
@@ -1,0 +1,40 @@
+module Kuiper.Kernel.GEMM.TensorCore2D.ProofSupport
+
+#lang-pulse
+
+open Kuiper
+#set-options "--ifuel 1 --initial_fuel 0 --max_fuel 1"
+#set-options "--z3rlimit 120"
+
+open Kuiper.EMatrix
+open Kuiper.EMatrix.Tiling
+open Kuiper.TensorCore
+open Pulse.Lib.Array
+
+let fragarrayA_approximates (#et:Type0) {| scalar et, real_like et |}
+  (#tm #tn #tk : pos)
+  (wm : nat)
+  (arr : array (fragment et FragA tm tn tk FragLRM) { Pulse.Lib.Array.length arr == wm})
+  (rm : chest2 real (wm*tm) tk)
+  : slprop
+  =
+    exists* (eAs : seq (chest2 et tm tk)).
+      arr |-> eAs **
+      pure (
+        (Seq.length eAs == wm) /\
+        forall (i : natlt wm).
+          (Seq.index eAs i) %~ (ematrix_subtile rm tm tk i 0))
+
+let fragarrayB_approximates (#et:Type0) {| scalar et, real_like et |}
+  (#tm #tn #tk : pos)
+  (wn : nat)
+  (arr : array (fragment et FragB tm tn tk FragLRM) { Pulse.Lib.Array.length arr == wn})
+  (rm : chest2 real tk (wn*tn))
+  : slprop
+  =
+    exists* (eBs : seq (chest2 et tk tn)).
+      arr |-> eBs **
+      pure (
+        (Seq.length eBs == wn) /\
+        forall (i : natlt wn).
+          (Seq.index eBs i) %~ (ematrix_subtile rm tk tn 0 i))
